\documentclass[11pt]{article}
\usepackage[T1]{fontenc}
\usepackage{geometry, changepage}
\usepackage{amsmath, amssymb, amsthm, bm}
\usepackage{physics}
\usepackage{hyperref}

\hypersetup{colorlinks=true, linkcolor=blue, urlcolor=cyan}
\setlength{\parindent}{0pt}
\setlength{\parskip}{5pt}

\newtheorem{theorem}{Theorem}
\newtheorem{lemma}{Lemma}
\newtheorem{claim}{Claim}
\newtheorem*{theorem*}{Theorem}
\newtheorem*{lemma*}{Lemma}
\newtheorem*{claim*}{Claim}

\title{Coset Properties}
\author{James Pagan}
\date{August 2023}

% --------------------------------------------- %

\begin{document}

\section{Group Cosets}

You can prove most of these in your head; it's just writing all these down is pretty useful.

\textbf{Basic Properties of Cosets}: If $H \subseteq G$ and $a, b \in G$ with $h \in H$,

\begin{itemize}

	\item $H(ab) = (Ha)b$ and $(ab)H = a(bH)$
	\item $|Ha| = |aH| = H$.
	\item $Ha = Hb$ or $Ha \cap Hb = \varnothing$; $aH = bH$ or $aH \cap bH = \varnothing$;

\end{itemize}

\textbf{Cosets and Subgroups}: If $N \trianglelefteq G$ and $H \subseteq G$ with $a, b \in G$,

\begin{itemize}

	\item $aNa^{-1} = N$ or $aNa^{-1} \subseteq N$.
	\item $aN = Na$.
	\item $Ha \subseteq Ga$ and $aH \subseteq aG$.

\end{itemize}

\textbf{Homomorphisms}: If $\varphi: G \rightarrow H$ is a homomorphism,

\begin{itemize}

	\item $\varphi(a)\varphi(H) = \varphi(aH)$ and $\varphi(H)\varphi(a) = \varphi(Ha)$

\end{itemize}

\newpage

\section{Ring Cosets}

For a ring $R$ with an ideal $I$ and an element $r \in R$, we define the coset of rings as follows: $r + I = \{ r + i \mid i \in I \}$.

\textbf{Basic Properties of Cosets}: If $I \trianglelefteq R$ and $r, j \in R$ with $i \in I$,

\begin{itemize}
	\item $I + (r + j) = (I + r) + j$ and $(r + j) + I = r + (j + I)$
	\item $r + I = I + r$.
	\item $I + r = I + j$ or $I + r \cap I + j = \varnothing$.
	\item $I + r = I + j \iff r - j \in I$.
\end{itemize}

\textbf{Homomorphisms}: If $\varphi: G \rightarrow H$ is a homomorphism,

\begin{itemize}
	\item $\varphi(r + I) = \varphi(r) + \varphi(I) = \varphi(I) + \varphi(r) = \varphi(I + r)$.
\end{itemize}

\end{document}
